Added support for Next Obligation

src/doctree.ml
@@ -58,9 +58,11 @@ class doctree =
   object(self)
     val doc : doc_node = doc_init
     val stack : grouping Stack.t = stack_init
-    val mutable last_definition : Style_group.body_node option = None
     val bullet_stack : Proof_bullet.t list ref Stack.t = Stack.create ()
+    val mutable suppress_proof = false
     initializer Stack.push (GBody doc_body_init) stack_init
+
+    method get_stack_length : int = Stack.length stack
 
     method load_style ~style = doc#get_style ~style ~ctx:[]
 
@@ -85,10 +87,13 @@ class doctree =
       | _ -> false
 
     method private is_proof proof_state expr =
-      match proof_state, expr with
-      | Some _, _
-      | _, VernacSubproof _ -> true
-      | _ -> false
+      if suppress_proof then false else begin
+        match proof_state, expr with
+        | Some _, _
+        | _, VernacExtend (("Obligations", 5), _)
+        | _, VernacSubproof _ -> true
+        | _ -> false
+      end
 
     method private is_end proof_state expr =
       match proof_state, expr with
@@ -99,14 +104,16 @@ class doctree =
 
     method add_vernac proof_state ({v = {control = _; attrs = _; expr}; loc = _} as v) =
       let _ : Proof.t option = proof_state in
-      let retain_last_definition = ref false in
+      if List.mem "definition" (as_grouping (Stack.top stack))#get_el.cls then begin
+        let is_sticky = self#is_proof proof_state expr in
+        if not is_sticky then ignore (Stack.pop stack)
+      end;
       if self#is_definition proof_state expr then begin
         let top_g = as_grouping (Stack.top stack) in
         let def_b = new Style_group.body_node ["definition"] in
-        last_definition <- Some def_b;
         def_b#add_child (new Style_vernac.vernac_node v);
         top_g#add_child ((def_b :> Style.node));
-        retain_last_definition := true
+        Stack.push (GBody def_b) stack;
       end else if self#is_module proof_state expr then begin
         let top_g = as_grouping (Stack.top stack) in
         let new_g = new Style_group.component_node ["module"] in
@@ -114,22 +121,18 @@ class doctree =
         Stack.push (GComponent new_g) stack;
         new_g#set_header (new Style_vernac.vernac_node v)
       end else if self#is_proof proof_state expr then begin
-        let last_g =
-          match last_definition with
-          | None -> as_grouping (Stack.top stack)
-          | Some g -> (g :> Style_group.grouping_node)
-        in
+        let top_g = as_grouping (Stack.top stack) in
         let new_g = new Style_group.component_node ["proof"] in
-        last_g#add_child (new_g :> Style.node);
+        top_g#add_child (new_g :> Style.node);
         Stack.push (GComponent new_g) stack;
         let _ =
           match expr with
+          | VernacExtend (("Obligations", 5), _)
           | VernacProof _
           | VernacSubproof _ -> new_g#set_header (new Style_vernac.vernac_node v)
           | _ -> new_g#add_child (new Style_vernac.vernac_node v)
         in
         Stack.push (ref []) bullet_stack;
-        retain_last_definition := true
       end else if self#is_bullet proof_state expr then begin
         let bullets = Stack.pop bullet_stack in
         let bullet = match expr with | VernacBullet b -> b | _ -> raise ExpectedBullet in
@@ -149,12 +152,14 @@ class doctree =
           ignore (Stack.pop stack)
         end done;
         let top_g = as_component (Stack.pop stack) in
-        (* remove all of the bullets from the stack *)
         top_g#set_footer (new Style_vernac.vernac_node v);
         if List.mem "proof" (top_g#get_el).cls then ignore (Stack.pop bullet_stack)
       end else begin
           let top_g = as_grouping (Stack.top stack) in
           top_g#add_child (new Style_vernac.vernac_node v)
       end;
-      if not (!retain_last_definition) then last_definition <- None
+      suppress_proof <-
+        match expr with
+        | VernacExtend (("Obligations", 5), _) -> true
+        | _ -> false
   end;;
