src/style_group.ml
@@ -26,13 +26,14 @@ class body_node cls =
     val mutable css_indent : int = 0
     val mutable css_betweenlines : int = 1
 
+    method set_css_indent x = css_indent <- x
+
     method! get_style ~style ~ctx =
       super#get_style ~style ~ctx;
       let _ = if List.mem "component" el.cls then css_indent <- 2 in
       let _ = if List.mem "definition" el.cls then css_betweenlines <- 0 in
       let _ = if List.mem "proof" el.cls then css_betweenlines <- 0 in
-      let _ = if List.mem "proof-bullet" el.cls then css_betweenlines <- 0 in
-      let _ = if List.mem "proof-bullet" el.cls then css_indent <- 0 in
+      let _ = if List.mem "proof-bullet" el.cls then begin css_betweenlines <- 0 ; css_indent <- 0 end in
       Queue.iter (fun n -> n#get_style ~style ~ctx:(el::ctx)) children
 
     method fmt ~ppf ~style ~ctx =
@@ -71,10 +72,12 @@ class component_node cls =
       | Some h, Some f ->
         let b : Style.node list = if body#has_children then [(body :> Style.node)] else [] in
         pp_open_vbox ppf 0;
+        (* pp_print_string ppf "full component";pp_print_cut ppf (); *)
         pp_print_list (fun ppf n -> n#fmt ~ppf ~style ~ctx:(el::ctx)) ppf ([h] @ b @ [f]);
         pp_close_box ppf ();
       | Some h, None ->
         pp_open_hbox ppf ();
+        (* pp_print_string ppf "header component";pp_print_cut ppf (); *)
         h#fmt ~ppf ~style ~ctx:(el::ctx);
         pp_print_space ppf ();
         body#fmt ~ppf ~style ~ctx:(el::ctx);
@@ -82,7 +85,11 @@ class component_node cls =
       | None, Some f ->
         let b : Style.node list = if body#has_children then [(body :> Style.node)] else [] in
         pp_open_vbox ppf 0;
+        (* pp_print_string ppf "footer component";pp_print_cut ppf (); *)
+        body#set_css_indent 0;
         pp_print_list (fun ppf n -> n#fmt ~ppf ~style ~ctx:(el::ctx)) ppf (b @ [f]);
         pp_close_box ppf ();
-      | None, None -> body#fmt ~ppf ~style ~ctx:(el::ctx)
+      | None, None ->
+        (* pp_print_string ppf "body component";pp_print_cut ppf (); *)
+        body#fmt ~ppf ~style ~ctx:(el::ctx)
     end;;
