src/style_group.mli
@@ -20,6 +20,8 @@ class body_node :
     method add_child : node -> unit
     method has_children : bool
 
+    method set_css_indent : int -> unit
+
     method get_style : style:Css.Types.Stylesheet.t -> ctx:context -> unit
 
     method fmt : ppf:Format.formatter -> style:Css.Types.Stylesheet.t -> ctx:context -> unit
